\section{Axiomas de estado sucesor}

\begin{itemize}

\item $\forall x,y$: posición(x,y,Resultado(acción,s)) $\Leftrightarrow$
\newline (acción = Mover(arriba) $\land$ posicion(x, SumarPosicion(y,-1),s))
\newline $\lor$
\newline (acción = Mover(abajo) $\land$ posicion(x, SumarPosicion(y,1),s))
\newline $\lor$
\newline (acción = Mover(derecha) $\land$ posicion(SumarPosicion(x,-1),y,s))
\newline $\lor$
\newline (acción = Mover(izquierda) $\land$ posicion(SumarPosicion(x,1),y,s))
\newline $\lor$
\newline (acción $\ne$ Mover(dirección) $\land$ posición(x,y,s))

\item $\forall x,y$: hayComida(x,y,Resultado(acción,s)) $\Leftrightarrow$
\newline (acción $\ne$ Comer $\land$ hayComida(x,y,s)

\item $\forall x,y$: hayEnemigo(x,y,Resultado(acción,s)) $\Leftrightarrow$
\newline (acción $\ne$ Pelear $\land$ hayEnemigo(x,y,s)

\end{itemize}

